A12Kernel/Proofs.lean
@@ -145,7 +145,7 @@ import A12Kernel.Proofs.AddressedNumberExtremum
 import A12Kernel.Proofs.AddressedNumberBinary
 import A12Kernel.Proofs.AddressedNumberDivision
 import A12Kernel.Proofs.AddressedNumberPower
-import A12Kernel.Proofs.AddressedNumericLeafConsumer
+import A12Kernel.Proofs.AddressedNumericOperationConsumer
 import A12Kernel.Proofs.NumberToStringComputationRun
 import A12Kernel.Proofs.StringToNumberComputationRun
 import A12Kernel.Proofs.ScalarComputationRun
